# WIP! https://soukai.noeldemartin.com/vocab/ doesn't exist yet.
# Based on https://github.com/schemaorg/schemaorg/blob/main/data/schema.ttl

@prefix : <https://soukai.noeldemartin.com/vocab/> .
@prefix rdf: <http://www.w3.org/1999/02/22-rdf-syntax-ns#> .
@prefix rdfs: <http://www.w3.org/2000/01/rdf-schema#> .
@prefix dcmi: <http://purl.org/dc/dcmitype/> .
@prefix xsd: <http://www.w3.org/2001/XMLSchema#dateTime> .

:Metadata a rdfs:Class ;
    rdfs:label "Metadata" ;
    rdfs:comment "Metadata about a resource." ;
    rdfs:subClassOf dcmi:Dataset .

:Operation a rdfs:Class ;
    rdfs:label "Operation" ;
    rdfs:comment "Operation performed on a resource." ;
    rdfs:subClassOf dcmi:Dataset .

:OperationType a rdf:Class ;
    rdfs:label "Operation Type" ;
    rdfs:comment "Type of the operation." .

:resource a rdf:Property ;
    rdfs:label "resource" ;
    rdfs:comment "If the object is a :Metadata, resource which the metadata makes reference to. If the object is a :Operation, resource affected by the operation." ;
    rdfs:subPropertyOf dcmi:subject ;
    rdfs:range rdfs:Resource ;
    rdfs:domain :Metadata, :Operation .

:createdAt a rdf:Property ;
    rdfs:label "createdAt" ;
    rdfs:comment "Time at which the resource was created." ;
    rdfs:subPropertyOf dcmi:created ;
    rdfs:range xsd:dateTime ;
    rdfs:domain :Metadata .

:updatedAt a rdf:Property ;
    rdfs:label "updatedAt" ;
    rdfs:comment "Time at which the resource was updated for the last time." ;
    rdfs:subPropertyOf dcmi:modified ;
    rdfs:range xsd:dateTime ;
    rdfs:domain :Metadata .

:deletedAt a rdf:Property ;
    rdfs:label "deletedAt" ;
    rdfs:comment "Time at which the resource was soft deleted." ;
    rdfs:range xsd:dateTime ;
    rdfs:domain :Metadata .

:type a rdf:Property ;
    rdfs:label "type" ;
    rdfs:comment "Type of the operation. If this property is missing, :SetOperation will be assumed." ;
    rdfs:range :OperationType ;
    rdfs:domain :Operation .

:property a rdf:Property ;
    rdfs:label "property" ;
    rdfs:comment "Property affected by the operation." ;
    rdfs:range rdf:Property ;
    rdfs:domain :Operation .

:value a rdf:Property ;
    rdfs:label "value" ;
    rdfs:comment "Value set by the operation." ;
    rdfs:domain :Operation .

:date a rdf:Property ;
    rdfs:label "date" ;
    rdfs:comment "Time at which the operation happened." ;
    rdfs:subPropertyOf dcmi:created ;
    rdfs:range xsd:dateTime ;
    rdfs:domain :Operation .

:SetOperation a :OperationType ;
    rdfs:label "Set Operation" ;
    rdfs:comment "A type of operation that removes all previous values for the affected property and replaces them with new ones." .

:UnsetOperation a :OperationType ;
    rdfs:label "Unset Operation" ;
    rdfs:comment "A type of operation that removes all previous values for the affected property." .

:AddOperation a :OperationType ;
    rdfs:label "Add Operation" ;
    rdfs:comment "A type of operation that adds new values to the affected property." .

:RemoveOperation a :OperationType ;
    rdfs:label "Remove Operation" ;
    rdfs:comment "A type of operation that removes previous values from the affected property." .
